\documentclass[12pt]{article}

\usepackage[english]{babel}
\usepackage[margin=0.8in]{geometry}

% Math/Greek packages
\usepackage{amssymb,amsmath,amsthm, mathtools} 
\usepackage{algorithm, algorithmic}
\usepackage{upgreek, siunitx}
\usepackage{setspace}

% Graphics/Presentation packages
\usepackage{graphicx}
\usepackage{cancel}
\usepackage{tabulary, enumitem, array}
\usepackage{xparse,mleftright,tikz}
\usepackage{physics}

% Misc packages
\usepackage{fancyhdr}


\usepackage[export]{adjustbox}

\usepackage{esint}

\sisetup{locale=US,group-separator = {,}}
\usepackage[colorlinks=true, allcolors=blue]{hyperref}


% Box function - update this as more sophisticated solutions are found
\newcommand\mybox[2][]{\tikz[overlay]\node[fill=blue!20,inner sep=2pt, anchor=text, rectangle, rounded corners=1mm,#1] {#2};\phantom{#2}}
\renewcommand{\arraystretch}{1.2}

% General macro declarations


\makeatletter
\let\oldabs\abs
\def\abs{\@ifstar{\oldabs}{\oldabs*}}
%
\let\oldnorm\norm
\def\norm{\@ifstar{\oldnorm}{\oldnorm*}}
\makeatother

	\begin{document}

\title{PHSX 491: HW02}
\author{William Jardee}
\maketitle

{\bf Thanks for the feedback on the last assignment about the margins. I realize that for homework the margin might have been a little bigger than ideal. I appreciate the feedback, so please keep them coming!}
\bigskip

The objective of this homework is show that 
\[\vec{A}\times (\vec{B}\times \vec{C}) = (\vec{A}\cdot \vec{C})\vec{B} - (\vec{A}\cdot \vec{B})\vec{C}\]
by using the Levi-Civita symbol and index notation.

\begin{enumerate}[label=\alph*)]
\item Show that $[\vec{A}\times \vec{B}]_i = \varepsilon_{ijk}A^jB^k$:\vspace{0.5em}

$[\vec{A} \times \vec{B}] = [A_y B_z - A_z B_y]\hat{x} - [A_x B_z - A_z B_x]\hat{y} + [A_x B_y - A_y B_x]\hat{z}$\vspace{0.5em}\\
$[\vec{A} \times \vec{B}]_x = A_y B_z - A_z B_y$\vspace{0.5em}\\
\hspace*{4.1em}$= \varepsilon_{xyz}A_y B_z + \varepsilon_{xzy}A_z B_y + \cancelto{0}{\varepsilon_{xxy}A_x B_y} + \cancelto{0}{...}$\vspace{0.5em}\\
\hspace*{4.1em}$=\varepsilon_{xjk}A^jB^k$\vspace{0.5em}\\
using a very similar logic:\vspace{0.5em}\\
$[\vec{A}\times \vec{B}]_y = A_z B_x - A_x B_z$\vspace{0.5em}\\
\hspace*{4.1em}$= \varepsilon_{yzx} A_z B_x + \varepsilon_{yxz}A_x B_z + \cancelto{0}{...}$\vspace{0.5em}\\
\hspace*{4.1em}$= \varepsilon_{yjk}A^j B^k$\vspace{0.5em}\\
$[\vec{A}\times \vec{B}]_z = \varepsilon_{zjk}A^j B^k$

So, putting all three of these together:

\[\boxed{[\vec{A}\times \vec{B}]_i = \varepsilon_{ijk}A^jB^k}\]

\item Show that $\varepsilon^{123} = 1$:\vspace{0.5em}

We know that there is the rule $g^{ij}A_i = A^j$, where $g$ is the metric of our space. For regular, Cartesian space:
\[g = \mqty[1 & 0 & 0 \\ 0& 1 & 0\\ 0 & 0 & 1]\]

Jumping to the conclusion:\vspace{0.5em}\\
$\varepsilon^{123} = g^{33}\varepsilon^{12}_{\hspace*{0.8em}3} = g^{33}g^{22}\varepsilon^1_{\hspace*{0.4em} 2 3} = g^{33}g^{22}g^{11}\varepsilon_{123}$\vspace{0.5em}\\
\hspace*{1.9em}$= 1 \cdot 1 \cdot 1 \cdot \varepsilon_{123} = 1 \quad \checkmark$

\item Write down the $i$th component of $\vec{A}\times (\vec{B} \times \vec{C})$ using index notation.:\vspace{0.5em}

$\vec{A}\times[\vec{B}\times \vec{C}]_i = \varepsilon_{ijk}A^j [\vec{B}\times \vec{C}]^k$\vspace{0.5em}\\
$g_{kk}g_{jj}g^{kk}g^{ii}g^{jj}\vec{A}\times[\vec{B}\times \vec{C}]_i = g_{kk}g_{jj}g^{kk}g^{ii}g^{jj}\varepsilon^{ijk}A^j [\vec{B}\times \vec{C}]^k$\vspace{0.5em}\\
$1 \cdot 1 \cdot 1 \cdot 1 \cdot 1 \cdot \vec{A}\times[\vec{B}\times \vec{C}]^i=\varepsilon^{ijk}A_j[\vec{B}\times \vec{C}]_k$\vspace{0.5em}\\
$\vec{A}\times[\vec{B}\times \vec{C}]^i =\varepsilon^{ijk}A_j \varepsilon_{kmn}B^m C^n$\vspace{0.5em}\\
\hspace*{6em}$=\varepsilon^{kij}\varepsilon_{kmn}A_jB^m C^n$

\[\boxed{[\vec{A}\times\vec{B}\times \vec{C}]^i = \varepsilon^{kij}\varepsilon_{kmn}A_jB^m C^n}\]

\item Write down the $i$th component of $(\vec{A}\cdot \vec{C})\vec{B} - (\vec{A}\cdot \vec{B})\vec{C}$ using index notation.:\vspace{0.5em}

\[\boxed{[(\vec{A}\cdot \vec{C})\vec{B} - (\vec{A} \cdot \vec{B})\vec{C}]^i = A^\alpha C_\alpha B_i - A^\alpha B_\alpha C_i}\]

\item Finish out showing that the two sides are equal:

Let's pick back up the left side:\vspace{0.5em}\\
$[\vec{A}\times\vec{B}\times \vec{C}]^i = \varepsilon^{kij}\varepsilon_{kmn}A_jB^m C^n$\vspace{0.5em}\\
\hspace*{6em}$= \left[\delta_m^i \delta_n^j - \delta_m^j \delta^i_n\right]A_jB^mC^n$\vspace{0.5em}\\
\hspace*{6em}$=\delta_m^i \delta_n^j A_jB^mC^n - \delta_m^j \delta^i_n A_jB^mC^n$\vspace{0.5em}\\
\hspace*{6em}$= A_nC^nB^i - A_mB^mC^i$\vspace{0.5em}\\
$g_{ii}[\vec{A}\times\vec{B}\times \vec{C}]^i = g_{ii} [A_nC^nB^i - A_mB^mC^i]$\vspace{0.5em}\\
\hspace*{7em}$= A_\alpha B^\alpha B_i - A_\alpha B^\alpha C_i$\vspace{0.5em}\\
\hspace*{7em}$=[(\vec{A}\cdot \vec{C})\vec{B} - (\vec{A} \cdot \vec{B})\vec{C}]^i $\vspace{0.5em}\\
Thus:

\[\boxed{\vec{A}\times[\vec{B}\times \vec{C}] = (\vec{A}\cdot \vec{C})\vec{B} - (\vec{A} \cdot \vec{B})\vec{C}}\]


\end{enumerate}


\end{document}